iris/ProofForkret.v
@@ -111,6 +111,7 @@ Section Res.
   Definition usertrap_res_pt_open := UC.usertrap_res_pt_open.
   Definition usertrap_res_bare_norm := UC.usertrap_res_bare_norm.
   Definition usertrap_res_csrs_open := UC.usertrap_res_csrs_open.
+  Definition usertrap_res_sstc := UC.usertrap_res_sstc.
   Definition usertrap_res_tf_csrs_open := UC.usertrap_res_tf_csrs_open.
   Definition usertrap_res_tf_open := UC.usertrap_res_tf_open.
 
