iris/ProofForkretPark.v
@@ -93,6 +93,7 @@ Section Res.
   Definition usertrap_res_pt_open := FR.usertrap_res_pt_open.
   Definition usertrap_res_bare_norm := FR.usertrap_res_bare_norm.
   Definition usertrap_res_csrs_open := FR.usertrap_res_csrs_open.
+  Definition usertrap_res_sstc := FR.usertrap_res_sstc.
   Definition usertrap_res_tf_csrs_open := FR.usertrap_res_tf_csrs_open.
   Definition usertrap_res_tf_open := FR.usertrap_res_tf_open.
 End Res.
